feat: add Cslib/Computability/Languages/RegularLanguage.lean and associated changes

Cslib/Computability/Automata/DA.lean
@@ -6,19 +6,52 @@ Authors: Fabrizio Montesi
 
 import Cslib.Computability.Automata.NA
 
-
-
 /-! # Deterministic Automaton
 
 A Deterministic Automaton (DA) is an automaton defined by a transition function.
+
+## References
+
+* [J. E. Hopcroft, R. Motwani, J. D. Ullman,
+  *Introduction to Automata Theory, Languages, and Computation*][Hopcroft2006]
 -/
 
 namespace Cslib
+
+open List
 
 structure DA (State : Type _) (Symbol : Type _) where
   /-- The initial state of the automaton. -/
   start : State
   /-- The transition function of the automaton. -/
   tr : State → Symbol → State
+
+namespace DA
+
+variable {State State1 State2 : Type _} {Symbol : Type _}
+
+/-- Extended transition function.
+
+Implementation note: compared to [Hopcroft2006], the definition consumes the input list of symbols
+from the left (instead of the right), in order to match the way lists are constructed.
+-/
+@[scoped grind =]
+def mtr (DA : DA State Symbol) (s : State) (xs : List Symbol) := xs.foldl DA.tr s
+
+@[simp, scoped grind =]
+theorem mtr_nil_eq {DA : DA State Symbol} {s : State} : DA.mtr s [] = s := rfl
+
+@[scoped grind =]
+def prod (da1 : DA State1 Symbol) (da2 : DA State2 Symbol) : DA (State1 × State2) Symbol where
+  start := (da1.start, da2.start)
+  tr := fun (s1, s2) x ↦ (da1.tr s1 x, da2.tr s2 x)
+
+@[simp, scoped grind =]
+theorem prod_mtr_eq (da1 : DA State1 Symbol) (da2 : DA State2 Symbol)
+    (s : State1 × State2) (xs : List Symbol) :
+    (da1.prod da2).mtr s xs = (da1.mtr s.fst xs, da2.mtr s.snd xs) := by
+  induction xs generalizing s <;> grind
+
+end DA
 
 end Cslib
