Cslib.lean
@@ -8,6 +8,7 @@ import Cslib.Computability.Automata.NFA
 import Cslib.Computability.Automata.NFAToDFA
 import Cslib.Computability.Languages.Language
 import Cslib.Computability.Languages.OmegaLanguage
+import Cslib.Computability.Languages.RegularLanguage
 import Cslib.Foundations.Control.Monad.Free
 import Cslib.Foundations.Control.Monad.Free.Effects
 import Cslib.Foundations.Control.Monad.Free.Fold
