Cslib/Computability/Languages/RegularLanguage.lean
@@ -1,0 +1,126 @@
+/-
+Copyright (c) 2025 Ching-Tsun Chou. All rights reserved.
+Released under Apache 2.0 license as described in the file LICENSE.
+Authors: Ching-Tsun Chou
+-/
+
+import Cslib.Computability.Automata.DFAToNFA
+import Cslib.Computability.Automata.NFAToDFA
+import Mathlib.Computability.DFA
+import Mathlib.Tactic
+
+/-!
+# Regular languages
+-/
+
+open Set Function
+open scoped Computability
+
+namespace Language
+
+variable {Symbol : Type _} [Finite Symbol]
+
+theorem regular_iff_cslib_dfa {l : Language Symbol} :
+    l.IsRegular ↔ ∃ State : Type, ∃ dfa : Cslib.DFA State Symbol, dfa.language = l := by
+  constructor
+  · rintro ⟨State, h_State, dfa, rfl⟩
+    let dfa' : Cslib.DFA State Symbol := {
+      start := dfa.start
+      tr := dfa.step
+      accept := dfa.accept
+      finite_state := Fintype.finite h_State
+      finite_symbol := by infer_instance }
+    use State, dfa'
+    rfl
+  · rintro ⟨State, dfa, rfl⟩
+    let dfa' : DFA Symbol State := {
+      start := dfa.start
+      step := dfa.tr
+      accept := dfa.accept }
+    have := dfa.finite_state
+    use State, (Fintype.ofFinite State), dfa'
+    rfl
+
+theorem regular_iff_cslib_nfa {l : Language Symbol} :
+    l.IsRegular ↔ ∃ State : Type, ∃ nfa : Cslib.NFA State Symbol, nfa.language = l := by
+  rw [regular_iff_cslib_dfa] ; constructor
+  · rintro ⟨State, dfa, rfl⟩
+    use State, dfa.toNFA
+    exact Cslib.DFA.toNFA_language_eq
+  · rintro ⟨State, nfa, rfl⟩
+    use (Set State), nfa.toDFA
+    exact Cslib.NFA.toDFA_language_eq
+
+open Cslib
+
+@[simp]
+theorem regular_compl {l : Language Symbol} (h : l.IsRegular) : (lᶜ).IsRegular := by
+  rw [regular_iff_cslib_dfa] at h ⊢
+  obtain ⟨State, dfa, rfl⟩ := h
+  use State, dfa.compl
+  simp
+
+@[simp]
+theorem regular_zero : (0 : Language Symbol).IsRegular := by
+  rw [regular_iff_cslib_dfa]
+  use Unit, DFA.zero
+  simp
+
+@[simp]
+theorem regular_one : (1 : Language Symbol).IsRegular := by
+  rw [regular_iff_cslib_dfa]
+  use Fin 2, DFA.one
+  simp
+
+@[simp]
+theorem regular_top : (⊤ : Language Symbol).IsRegular := by
+  have : (⊥ᶜ : Language Symbol).IsRegular := regular_compl <| regular_zero (Symbol := Symbol)
+  rwa [← compl_bot]
+
+@[simp]
+theorem regular_inf {l1 l2 : Language Symbol}
+    (h1 : l1.IsRegular) (h2 : l2.IsRegular) : (l1 ⊓ l2).IsRegular := by
+  rw [regular_iff_cslib_dfa] at h1 h2 ⊢
+  obtain ⟨State1, dfa1, rfl⟩ := h1
+  obtain ⟨State2, dfa2, rfl⟩ := h2
+  use (State1 × State2), (dfa1.inf dfa2)
+  simp
+
+@[simp]
+theorem regular_add {l1 l2 : Language Symbol}
+    (h1 : l1.IsRegular) (h2 : l2.IsRegular) : (l1 + l2).IsRegular := by
+  rw [regular_iff_cslib_dfa] at h1 h2 ⊢
+  obtain ⟨State1, dfa1, rfl⟩ := h1
+  obtain ⟨State2, dfa2, rfl⟩ := h2
+  use (State1 × State2), (dfa1.add dfa2)
+  simp
+
+@[simp]
+theorem regular_iInf {I : Type _} [Finite I] {s : Set I} {l : I → Language Symbol}
+    (h : ∀ i ∈ s, (l i).IsRegular) : (⨅ i ∈ s, l i).IsRegular := by
+  generalize h_n : s.ncard = n
+  induction n generalizing s
+  case zero =>
+    obtain ⟨rfl⟩ := (ncard_eq_zero (s := s)).mp h_n
+    simp only [mem_empty_iff_false, not_false_eq_true, iInf_neg, iInf_top]
+    exact regular_top
+  case succ n h_ind =>
+    obtain ⟨i, t, h_i, rfl, rfl⟩ := (ncard_eq_succ (s := s)).mp h_n
+    rw [biInf_insert]
+    apply regular_inf <;> grind
+
+@[simp]
+theorem regular_iSup {I : Type _} [Finite I] {s : Set I} {l : I → Language Symbol}
+    (h : ∀ i ∈ s, (l i).IsRegular) : (⨆ i ∈ s, l i).IsRegular := by
+  generalize h_n : s.ncard = n
+  induction n generalizing s
+  case zero =>
+    obtain ⟨rfl⟩ := (ncard_eq_zero (s := s)).mp h_n
+    simp only [mem_empty_iff_false, not_false_eq_true, iSup_neg, iSup_bot]
+    exact regular_zero
+  case succ n h_ind =>
+    obtain ⟨i, t, h_i, rfl, rfl⟩ := (ncard_eq_succ (s := s)).mp h_n
+    rw [biSup_insert]
+    apply regular_add <;> grind
+
+end Language
